Versions/Bookmarker.i.dfy
@@ -8,6 +8,9 @@ module Bookmarker {
   import JournalChain
   import SM = MapSpec
   import opened VersionOp
+  import opened Options
+  import opened Journal
+  import opened Sequences
 
   import UI
 
@@ -27,97 +30,300 @@ module Bookmarker {
     && JournalChain.Init(k.jc, s.jc)
   }
 
-  predicate SendPersistentLoc(k: Constants, s: Variables, s': Variables, vop: VOp, uiop: UI.Op)
-  {
-    && uiop.NoOp?
-    && vop.SendPersistentLocOp?
-    && TriStateMap.Next(k.tsm, s.tsm, s'.tsm, vop)
-    && JournalChain.Next(k.jc, s.jc, s'.jc, vop)
-  }
-
-  predicate Advance(k: Constants, s: Variables, s': Variables, vop: VOp, uiop: UI.Op)
-  {
-    && vop.AdvanceOp?
-    && (vop.replay ==> uiop.NoOp?)
-    && (!vop.replay ==> vop.uiop == uiop)
-    && TriStateMap.Next(k.tsm, s.tsm, s'.tsm, vop)
-    && JournalChain.Next(k.jc, s.jc, s'.jc, vop)
-  }
-
-  predicate Crash(k: Constants, s: Variables, s': Variables, vop: VOp, uiop: UI.Op)
-  {
-    && vop.CrashOp?
-    && uiop.CrashOp?
-    && TriStateMap.Next(k.tsm, s.tsm, s'.tsm, vop)
-    && JournalChain.Next(k.jc, s.jc, s'.jc, vop)
-  }
-
-  predicate Freeze(k: Constants, s: Variables, s': Variables, vop: VOp, uiop: UI.Op)
-  {
-    && vop.FreezeOp?
-    && uiop.CrashOp?
-    && TriStateMap.Next(k.tsm, s.tsm, s'.tsm, vop)
-    && JournalChain.Next(k.jc, s.jc, s'.jc, vop)
-  }
-
-  predicate TristateInternal(k: Constants, s: Variables, s': Variables, vop: VOp, uiop: UI.Op)
-  {
-    && vop.TristateInternalOp?
-    && TriStateMap.Next(k.tsm, s.tsm, s'.tsm, vop)
-    && s'.jc == s.jc
-  }
-
-  predicate JournalInternal(k: Constants, s: Variables, s': Variables, vop: VOp, uiop: UI.Op)
-  {
-    && vop.JournalInternalOp?
-    && s'.tsm == s.tsm
-    && JournalChain.Next(k.jc, s.jc, s'.jc, vop)
-  }
-
-  predicate SendFrozenLoc(k: Constants, s: Variables, s': Variables, vop: VOp, uiop: UI.Op)
-  {
-    && vop.SendFrozenLocOp?
-    && TriStateMap.Next(k.tsm, s.tsm, s'.tsm, vop)
-    && JournalChain.Next(k.jc, s.jc, s'.jc, vop)
-  }
-
-  predicate ForgetOld(k: Constants, s: Variables, s': Variables, vop: VOp, uiop: UI.Op)
-  {
-    && vop.ForgetOldOp?
-    && TriStateMap.Next(k.tsm, s.tsm, s'.tsm, vop)
-    && JournalChain.Next(k.jc, s.jc, s'.jc, vop)
-  }
-
-  predicate PushSync(k: Constants, s: Variables, s': Variables, vop: VOp, uiop: UI.Op)
-  {
-    && vop.PushSyncOp?
-    && TriStateMap.Next(k.tsm, s.tsm, s'.tsm, vop)
-    && JournalChain.Next(k.jc, s.jc, s'.jc, vop)
-  }
-
-  predicate PopSync(k: Constants, s: Variables, s': Variables, vop: VOp, uiop: UI.Op)
-  {
-    && vop.PopSyncOp?
-    && TriStateMap.Next(k.tsm, s.tsm, s'.tsm, vop)
-    && JournalChain.Next(k.jc, s.jc, s'.jc, vop)
-  }
-
   predicate NextStep(k: Constants, s: Variables, s': Variables, vop: VOp, uiop: UI.Op)
   {
-    && (vop.SendPersistentLocOp? ==> SendPersistentLoc(k, s, s', vop, uiop))
-    && (vop.AdvanceOp? ==> Advance(k, s, s', vop, uiop))
-    && (vop.CrashOp? ==> Crash(k, s, s', vop, uiop))
-    && (vop.FreezeOp? ==> Freeze(k, s, s', vop, uiop))
-    && (vop.TristateInternalOp? ==> TristateInternal(k, s, s', vop, uiop))
-    && (vop.JournalInternalOp? ==> JournalInternal(k, s, s', vop, uiop))
-    && (vop.SendFrozenLocOp? ==> SendFrozenLoc(k, s, s', vop, uiop))
-    && (vop.ForgetOldOp? ==> ForgetOld(k, s, s', vop, uiop))
-    && (vop.PushSyncOp? ==> PushSync(k, s, s', vop, uiop))
-    && (vop.PopSyncOp? ==> PopSync(k, s, s', vop, uiop))
+    && TriStateMap.Next(k.tsm, s.tsm, s'.tsm, vop)
+    && JournalChain.Next(k.jc, s.jc, s'.jc, vop)
+    && VOpAgreesUIOp(vop, uiop)
   }
 
   predicate Next(k: Constants, s: Variables, s': Variables, uiop: UI.Op)
   {
     exists step: Step :: NextStep(k, s, s', step.vop, uiop)
+  }
+
+  ////
+  //// Lemmas about applying stuff to states.
+
+  function Apply(m: SM.Variables, je: JournalEntry) : SM.Variables
+  {
+    SM.Variables(m.view[je.key := je.value])
+  }
+
+  function ApplySeq(m: SM.Variables, jes: seq<JournalEntry>) : SM.Variables
+  {
+    if jes == [] then
+      m
+    else
+      Apply(ApplySeq(m, DropLast(jes)), Last(jes))
+  }
+
+  lemma ApplySeqAdditive(m: SM.Variables, a: seq<JournalEntry>,
+      b: seq<JournalEntry>)
+  ensures ApplySeq(m, a+b) == ApplySeq(ApplySeq(m, a), b)
+  {
+    if b == [] {
+      calc {
+        ApplySeq(m, a+b);
+        { assert a + b == a; }
+        ApplySeq(m, a);
+        ApplySeq(ApplySeq(m, a), []);
+        ApplySeq(ApplySeq(m, a), b);
+      }
+    } else {
+      calc {
+        ApplySeq(m, a+b);
+        Apply(ApplySeq(m, DropLast(a + b)), Last(a + b));
+        {
+          assert DropLast(a + b) == a + DropLast(b);
+          assert Last(a + b) == Last(b);
+        }
+        Apply(ApplySeq(m, a + DropLast(b)), Last(b));
+        {
+          ApplySeqAdditive(m, a, DropLast(b));
+        }
+        Apply(ApplySeq(ApplySeq(m, a), DropLast(b)), Last(b));
+        ApplySeq(ApplySeq(m, a), b);
+      }
+    }
+  }
+
+  lemma ApplySeqPrepend(k: SM.Constants, m: SM.Variables, uiop: UI.Op, m': SM.Variables, j: seq<JournalEntry>)
+  requires SM.Next(k, m, m', uiop)
+  ensures ApplySeq(m, JournalEntriesForUIOp(uiop) + j)
+       == ApplySeq(m', j)
+  {
+    assert m' == ApplySeq(m, JournalEntriesForUIOp(uiop));
+    ApplySeqAdditive(m, JournalEntriesForUIOp(uiop), j);
+  }
+
+  lemma ApplySeqAppend(k: SM.Constants, m: SM.Variables, j: seq<JournalEntry>, uiop: UI.Op, m': SM.Variables)
+  requires SM.Next(k, ApplySeq(m, j), m', uiop)
+  ensures ApplySeq(m, j + JournalEntriesForUIOp(uiop)) == m'
+
+  //// Inv definition
+
+  function {:opaque} JournalSlice(s: Variables, a: int, b: int) : (res : seq<JournalEntry>)
+  requires 0 <= a - s.jc.startVersion <= |s.jc.journal|
+  requires 0 <= b - s.jc.startVersion <= |s.jc.journal|
+  requires a <= b
+  ensures |res| == b - a
+  {
+    s.jc.journal[a - s.jc.startVersion .. b - s.jc.startVersion]
+  }
+
+  function {:opaque} JournalSuffix(s: Variables, a: int) : (res : seq<JournalEntry>)
+  requires 0 <= a - s.jc.startVersion <= |s.jc.journal|
+  ensures |res| == |s.jc.journal| - (a - s.jc.startVersion)
+  {
+    s.jc.journal[a - s.jc.startVersion ..]
+  }
+
+  function JournalForPersistent(s: Variables) : seq<JournalEntry>
+  requires 0 <= s.jc.persistentStateIndex - s.jc.startVersion <= |s.jc.journal|
+  {
+    JournalSuffix(s, s.jc.persistentStateIndex)
+  }
+
+  predicate StatesConsistent(
+      s: Variables,
+      m: SM.Variables,
+      m': SM.Variables,
+      v1: int, v2: int)
+  requires 0 <= v1 - s.jc.startVersion <= |s.jc.journal|
+  requires 0 <= v2 - s.jc.startVersion <= |s.jc.journal|
+  requires v1 <= v2
+  {
+    ApplySeq(m, JournalSlice(s, v1, v2)) == m'
+  }
+
+  predicate Inv(k: Constants, s: Variables)
+  {
+    && (s.jc.frozenLoc.Some? ==>
+      && s.tsm.frozenLoc == s.jc.frozenLoc
+    )
+    && (s.tsm.persistentLoc.Some? ==>
+      || s.tsm.persistentLoc.value == s.jc.persistentLoc
+      || s.tsm.frozenLoc == Some(s.jc.persistentLoc)
+    )
+    && (s.tsm.frozenLoc.Some? ==>
+      && s.tsm.frozenLoc.value in s.tsm.disk
+      && s.tsm.frozenState.Some?
+      && s.tsm.disk[s.tsm.frozenLoc.value]
+          == s.tsm.frozenState.value
+    )
+    && (s.jc.frozenStateIndex.Some? <==> s.tsm.frozenState.Some?)
+    && (s.tsm.frozenState.Some? ==>
+      s.tsm.ephemeralState.Some?
+    )
+    && (s.tsm.ephemeralState.Some? ==>
+      s.tsm.persistentLoc.Some?
+    )
+    && s.jc.persistentLoc in s.tsm.disk
+    && s.jc.startVersion <= s.jc.persistentStateIndex
+    && s.jc.persistentStateIndex <= s.jc.persistentJournalIndex
+    && s.jc.persistentStateIndex <= s.jc.ephemeralStateIndex
+    && (s.jc.frozenStateIndex.Some? ==> (
+      s.jc.persistentStateIndex
+        <= s.jc.frozenStateIndex.value
+        <= s.jc.ephemeralStateIndex
+    ))
+    && s.jc.persistentJournalIndex <= s.jc.startVersion + |s.jc.journal|
+    && s.jc.ephemeralStateIndex <= s.jc.startVersion + |s.jc.journal|
+
+    && var persistentState := s.tsm.disk[s.jc.persistentLoc];
+    && (s.tsm.ephemeralState.Some? ==>
+      StatesConsistent(s,
+          persistentState, s.tsm.ephemeralState.value,
+          s.jc.persistentStateIndex, s.jc.ephemeralStateIndex)
+    )
+    && (s.jc.frozenStateIndex.Some? ==>
+      && StatesConsistent(s,
+          persistentState, s.tsm.frozenState.value,
+          s.jc.persistentStateIndex, s.jc.frozenStateIndex.value)
+      && StatesConsistent(s,
+          s.tsm.frozenState.value, s.tsm.ephemeralState.value,
+          s.jc.frozenStateIndex.value, s.jc.ephemeralStateIndex)
+    )
+  }
+
+  lemma InitImpliesInv(k: Constants, s: Variables, s': Variables)
+  requires Init(k, s)
+  ensures Inv(k, s)
+  {
+  }
+
+  lemma JournalSliceAppend(k: Constants, s: Variables, s': Variables, vop: VOp, i: int)
+  requires Inv(k, s)
+  requires JournalChain.Next(k.jc, s.jc, s'.jc, vop)
+  requires vop.AdvanceOp?
+  requires 0 <= i - s.jc.startVersion <= |s.jc.journal|
+  requires 0 <= s.jc.ephemeralStateIndex - s.jc.startVersion <= |s.jc.journal|
+  requires i <= s.jc.ephemeralStateIndex
+  ensures JournalSlice(s', i, s'.jc.ephemeralStateIndex)
+        == JournalSlice(s, i, s.jc.ephemeralStateIndex)
+            + JournalEntriesForUIOp(vop.uiop)
+  {
+    reveal_JournalSlice();
+    if JournalChain.AdvanceEphemeral(k.jc, s.jc, s'.jc, vop) {
+      assert JournalSlice(s', i, s'.jc.ephemeralStateIndex)
+            == JournalSlice(s, i, s.jc.ephemeralStateIndex)
+                + JournalEntriesForUIOp(vop.uiop);
+    } else if JournalChain.Replay(k.jc, s.jc, s'.jc, vop) {
+      assert JournalSlice(s', i, s'.jc.ephemeralStateIndex)
+            == JournalSlice(s, i, s.jc.ephemeralStateIndex)
+                + JournalEntriesForUIOp(vop.uiop);
+    }
+  }
+
+  lemma JournalSliceAppendPersistent(k: Constants, s: Variables, s': Variables, vop: VOp)
+  requires Inv(k, s)
+  requires JournalChain.Next(k.jc, s.jc, s'.jc, vop)
+  requires vop.AdvanceOp?
+  ensures JournalSlice(s', s'.jc.persistentStateIndex, s'.jc.ephemeralStateIndex)
+        == JournalSlice(s, s.jc.persistentStateIndex, s.jc.ephemeralStateIndex)
+            + JournalEntriesForUIOp(vop.uiop)
+  {
+    JournalSliceAppend(k, s, s', vop, s.jc.persistentStateIndex);
+  }
+
+  lemma JournalSliceAppendFrozen(k: Constants, s: Variables, s': Variables, vop: VOp)
+  requires Inv(k, s)
+  requires JournalChain.Next(k.jc, s.jc, s'.jc, vop)
+  requires vop.AdvanceOp?
+  requires s'.jc.frozenStateIndex.Some?
+  ensures JournalSlice(s', s'.jc.frozenStateIndex.value, s'.jc.ephemeralStateIndex)
+        == JournalSlice(s, s.jc.frozenStateIndex.value, s.jc.ephemeralStateIndex)
+            + JournalEntriesForUIOp(vop.uiop)
+  {
+    JournalSliceAppend(k, s, s', vop, s.jc.frozenStateIndex.value);
+  }
+  
+  lemma AdvancePreservesInv(k: Constants, s: Variables, s': Variables, vop: VOp, uiop: UI.Op)
+  requires NextStep(k, s, s', vop, uiop)
+  requires vop.AdvanceOp?
+  requires Inv(k, s)
+  ensures Inv(k, s')
+  {
+    var tsm_step :| TriStateMap.NextStep(k.tsm, s.tsm, s'.tsm, vop, tsm_step);
+    var jc_step :| JournalChain.NextStep(k.jc, s.jc, s'.jc, vop, jc_step);
+    var persistentState := s.tsm.disk[s.jc.persistentLoc];
+
+    ApplySeqAppend(k.tsm.k, persistentState, 
+        JournalSlice(s, s.jc.persistentStateIndex, s.jc.ephemeralStateIndex),
+        vop.uiop, s'.tsm.ephemeralState.value);
+    JournalSliceAppendPersistent(k, s, s', vop);
+
+    if s.jc.frozenStateIndex.Some? {
+      assert JournalSlice(s', s'.jc.persistentStateIndex, s'.jc.frozenStateIndex.value)
+          == JournalSlice(s, s.jc.persistentStateIndex, s.jc.frozenStateIndex.value)
+              by { reveal_JournalSlice(); }
+
+      ApplySeqAppend(k.tsm.k, s.tsm.frozenState.value, 
+          JournalSlice(s, s.jc.frozenStateIndex.value, s.jc.ephemeralStateIndex),
+          vop.uiop, s'.tsm.ephemeralState.value);
+      JournalSliceAppendFrozen(k, s, s', vop);
+    }
+
+    if JournalChain.AdvanceEphemeral(k.jc, s.jc, s'.jc, vop) {
+      assert Inv(k, s');
+    } else if JournalChain.Replay(k.jc, s.jc, s'.jc, vop) {
+      assert Inv(k, s');
+    }
+  }
+
+  lemma NextStepPreservesInv(k: Constants, s: Variables, s': Variables, vop: VOp, uiop: UI.Op)
+  requires NextStep(k, s, s', vop, uiop)
+  requires Inv(k, s)
+  ensures Inv(k, s')
+  {
+    reveal_JournalSlice();
+
+    var tsm_step :| TriStateMap.NextStep(k.tsm, s.tsm, s'.tsm, vop, tsm_step);
+    var jc_step :| JournalChain.NextStep(k.jc, s.jc, s'.jc, vop, jc_step);
+
+    var persistentState := s.tsm.disk[s.jc.persistentLoc];
+
+    match vop {
+      case SendPersistentLocOp(loc) => { }
+      case AdvanceOp(_, _) => {
+        AdvancePreservesInv(k, s, s', vop, uiop);
+      }
+      case CrashOp => {
+        assert JournalChain.Crash(k.jc, s.jc, s'.jc, vop);
+        assert TriStateMap.Crash(k.tsm, s.tsm, s'.tsm, vop);
+      }
+      case FreezeOp => { }
+      case TristateInternalOp => { }
+      case JournalInternalOp => {
+        assert s.tsm == s'.tsm;
+        if JournalChain.AdvancePersistent(k.jc, s.jc, s'.jc, vop) {
+          assert Inv(k, s');
+        }
+        else if JournalChain.CleanUpStep(k.jc, s.jc, s'.jc, vop) {
+          assert Inv(k, s');
+        }
+        else {
+          assert s.jc == s'.jc;
+        }
+      }
+      case SendFrozenLocOp(loc) => { }
+      case ForgetOldOp => {
+        assert JournalChain.ForgetOld(k.jc, s.jc, s'.jc, vop);
+        assert TriStateMap.ForgetOld(k.tsm, s.tsm, s'.tsm, vop);
+        assert Inv(k, s');
+      }
+      case PushSyncOp(id) => { }
+      case PopSyncOp(id) => { }
+    }
+  }
+
+  lemma NextPreservesInv(k: Constants, s: Variables, s': Variables, uiop: UI.Op)
+  requires Next(k, s, s', uiop)
+  requires Inv(k, s)
+  ensures Inv(k, s')
+  {
+    var step: Step :| NextStep(k, s, s', step.vop, uiop);
+    NextStepPreservesInv(k, s, s', step.vop, uiop);
   }
 }
