Versions/VOp.i.dfy
@@ -17,8 +17,26 @@ module VersionOp {
     | PushSyncOp(ghost id: int)
     | PopSyncOp(ghost id: int)
 
-  predicate VOpAgreesUIOp(vop: VOp, uiop: UIOp)
+  predicate VOpAgreesUIOp(vop: VOp, uiop: UI.Op)
   {
-    && (vop
+    && (vop.SendPersistentLocOp? ==> uiop.NoOp?)
+    && (vop.AdvanceOp? ==>
+        && (vop.replay ==> uiop.NoOp?)
+        && (!vop.replay ==> uiop == vop.uiop)
+    )
+    && (vop.CrashOp? ==> uiop.CrashOp?)
+    && (vop.FreezeOp? ==> uiop.NoOp?)
+    && (vop.TristateInternalOp? ==> uiop.NoOp?)
+    && (vop.JournalInternalOp? ==> uiop.NoOp?)
+    && (vop.SendFrozenLocOp? ==> uiop.NoOp?)
+    && (vop.ForgetOldOp? ==> uiop.NoOp?)
+    && (vop.PushSyncOp? ==>
+      && uiop.PushSyncOp?
+      && uiop.id == vop.id
+    )
+    && (vop.PopSyncOp? ==>
+      && uiop.PopSyncOp?
+      && uiop.id == vop.id
+    )
   }
 }
