Versions/Bookmarker_Refines_FullVersionedMap.i.dfy
@@ -1,0 +1,282 @@
+include "Bookmarker.i.dfy"
+include "../MapSpec/FullVersionedMap.s.dfy"
+
+module Bookmarker_Refines_FullVersionedMap {
+  import Bookmarker
+  import FVM = FullVersionedMap
+  import opened Options
+  import opened Sequences
+  import opened Journal
+  import opened VersionOp
+  import MapSpec
+  import JournalChain
+
+  function statesOf(m: MapSpec.Variables, jes: seq<JournalEntry>) : (res : seq<MapSpec.Variables>)
+  ensures |res| == |jes| + 1
+  ensures res[0] == m
+  {
+    if jes == [] then
+      [m]
+    else
+      var p := statesOf(m, DropLast(jes));
+      var m' := Last(p);
+      var m1 := Bookmarker.Apply(m', Last(jes));
+      p + [m1]
+  }
+
+  lemma Last_statesOf_ApplySeq(m: MapSpec.Variables, jes: seq<JournalEntry>)
+  ensures Last(statesOf(m, jes)) == Bookmarker.ApplySeq(m, jes)
+
+  function Ik(k: Bookmarker.Constants) : FVM.Constants
+  {
+    FVM.Constants(k.tsm.k)
+  }
+
+  function persistentState(k: Bookmarker.Constants, s: Bookmarker.Variables) : MapSpec.Variables
+  requires Bookmarker.Inv(k, s)
+  {
+    s.tsm.disk[s.jc.persistentLoc]
+  }
+
+  function {:opaque} states(k: Bookmarker.Constants, s: Bookmarker.Variables)
+      : (res : seq<MapSpec.Variables>)
+  requires Bookmarker.Inv(k, s)
+  ensures |res| == |s.jc.journal| + 1
+      - (s.jc.persistentJournalIndex - s.jc.startVersion)
+  {
+    statesOf(persistentState(k, s), Bookmarker.JournalForPersistent(s))
+        [s.jc.persistentJournalIndex - s.jc.persistentStateIndex ..]
+  }
+
+  function I(k: Bookmarker.Constants, s: Bookmarker.Variables) : FVM.Variables
+  requires Bookmarker.Inv(k, s)
+  {
+    FVM.Variables(
+      s.jc.persistentJournalIndex,
+      states(k, s),
+      s.jc.syncReqs
+    )
+  }
+
+  lemma RefinesInit(k: Bookmarker.Constants, s: Bookmarker.Variables)
+    requires Bookmarker.Init(k, s)
+    ensures FVM.Init(Ik(k), I(k, s))
+  {
+    Bookmarker.reveal_JournalSuffix();
+    reveal_states();
+  }
+
+  lemma SendPersistentLocRefines(k: Bookmarker.Constants, s: Bookmarker.Variables, s':Bookmarker.Variables, uiop: UI.Op, vop: VOp)
+    requires Bookmarker.Inv(k, s)
+    requires Bookmarker.Inv(k, s')
+    requires Bookmarker.NextStep(k, s, s', vop, uiop)
+    requires vop.SendPersistentLocOp?
+    ensures FVM.Next(Ik(k), I(k, s), I(k, s'), uiop)
+  {
+    assert I(k, s).version == I(k, s').version;
+    assert Bookmarker.JournalForPersistent(s)
+        == Bookmarker.JournalForPersistent(s') by {
+      Bookmarker.reveal_JournalSuffix();
+    } 
+    assert I(k, s).states == I(k, s').states by {
+      assert persistentState(k, s) == persistentState(k, s');
+      reveal_states();
+    }
+    assert FVM.NextStep(Ik(k), I(k, s), I(k, s'), uiop, FVM.StutterStep);
+  }
+
+  lemma ephemeralIsLast(k: Bookmarker.Constants, s: Bookmarker.Variables)
+  requires s.jc.ephemeralStateIndex == s.jc.startVersion + |s.jc.journal|
+  requires s.tsm.ephemeralState.Some?
+  requires Bookmarker.Inv(k, s)
+  ensures s.tsm.ephemeralState.value == Last(I(k, s).states);
+  {
+    calc {
+      s.tsm.ephemeralState.value;
+      Bookmarker.ApplySeq(persistentState(k, s), Bookmarker.JournalSlice(s, s.jc.persistentStateIndex, s.jc.ephemeralStateIndex));
+      {
+        Bookmarker.reveal_JournalSlice();
+        Bookmarker.reveal_JournalSuffix();
+        assert Bookmarker.JournalSlice(s, s.jc.persistentStateIndex, s.jc.ephemeralStateIndex)
+            == Bookmarker.JournalForPersistent(s);
+      }
+      Bookmarker.ApplySeq(persistentState(k, s), Bookmarker.JournalForPersistent(s));
+      {
+        Last_statesOf_ApplySeq(persistentState(k, s), Bookmarker.JournalForPersistent(s));
+      }
+      Last(statesOf(persistentState(k, s), Bookmarker.JournalForPersistent(s)));
+      {
+        reveal_states();
+      }
+      Last(I(k, s).states);
+    }
+  }
+
+  lemma AdvanceRefines(k: Bookmarker.Constants, s: Bookmarker.Variables, s':Bookmarker.Variables, uiop: UI.Op, vop: VOp)
+    requires Bookmarker.Inv(k, s)
+    requires Bookmarker.Inv(k, s')
+    requires Bookmarker.NextStep(k, s, s', vop, uiop)
+    requires vop.AdvanceOp?
+    ensures FVM.Next(Ik(k), I(k, s), I(k, s'), uiop)
+  {
+    Bookmarker.reveal_JournalSuffix();
+
+    if JournalChain.AdvanceEphemeral(k.jc, s.jc, s'.jc, vop) {
+      assert MapSpec.Next(k.tsm.k,
+        s.tsm.ephemeralState.value,
+        s'.tsm.ephemeralState.value,
+        uiop);
+
+      assert Bookmarker.JournalForPersistent(s)
+          == Bookmarker.JournalSlice(s, s.jc.persistentStateIndex, s.jc.ephemeralStateIndex)
+        by {
+          Bookmarker.reveal_JournalSlice();
+        }
+
+      ephemeralIsLast(k, s);
+
+      var jes := JournalEntriesForUIOp(uiop);
+      if |jes| == 0 {
+        assert s'.jc.journal == s.jc.journal;
+        assert s == s';
+        assert I(k, s) == I(k, s');
+        Last_statesOf_ApplySeq(persistentState(k, s), Bookmarker.JournalForPersistent(s));
+        assert FVM.Query(Ik(k), I(k, s), I(k, s'), uiop);
+        assert FVM.NextStep(Ik(k), I(k, s), I(k, s'), uiop, FVM.QueryStep);
+      } else if |jes| == 1 {
+        assert DropLast(Bookmarker.JournalForPersistent(s')) == Bookmarker.JournalForPersistent(s);
+        assert Last(Bookmarker.JournalForPersistent(s')) == jes[0];
+
+        assert Bookmarker.JournalForPersistent(s')
+            == Bookmarker.JournalSlice(s', s'.jc.persistentStateIndex, s'.jc.ephemeralStateIndex)
+          by { Bookmarker.reveal_JournalSlice(); }
+
+        ephemeralIsLast(k, s');
+
+        reveal_states();
+
+        assert FVM.Advance(Ik(k), I(k, s), I(k, s'), uiop);
+        assert FVM.NextStep(Ik(k), I(k, s), I(k, s'), uiop, FVM.AdvanceStep);
+      } else {
+        assert false;
+      }
+
+    } else if JournalChain.Replay(k.jc, s.jc, s'.jc, vop) {
+      reveal_states();
+      assert FVM.NextStep(Ik(k), I(k, s), I(k, s'), uiop, FVM.StutterStep);
+    } else {
+      assert false;
+    }
+  }
+
+  lemma CrashRefines(k: Bookmarker.Constants, s: Bookmarker.Variables, s':Bookmarker.Variables, uiop: UI.Op, vop: VOp)
+    requires Bookmarker.Inv(k, s)
+    requires Bookmarker.Inv(k, s')
+    requires Bookmarker.NextStep(k, s, s', vop, uiop)
+    requires vop.CrashOp?
+    ensures FVM.Next(Ik(k), I(k, s), I(k, s'), uiop)
+  {
+    assert FVM.Crash(Ik(k), I(k, s), I(k, s'), uiop);
+    assert FVM.NextStep(Ik(k), I(k, s), I(k, s'), uiop, FVM.CrashStep);
+  }
+
+  lemma FreezeRefines(k: Bookmarker.Constants, s: Bookmarker.Variables, s':Bookmarker.Variables, uiop: UI.Op, vop: VOp)
+    requires Bookmarker.Inv(k, s)
+    requires Bookmarker.Inv(k, s')
+    requires Bookmarker.NextStep(k, s, s', vop, uiop)
+    requires vop.FreezeOp?
+    ensures FVM.Next(Ik(k), I(k, s), I(k, s'), uiop)
+  {
+    assert FVM.NextStep(Ik(k), I(k, s), I(k, s'), uiop, FVM.StutterStep);
+  }
+
+  lemma TristateInternalRefines(k: Bookmarker.Constants, s: Bookmarker.Variables, s':Bookmarker.Variables, uiop: UI.Op, vop: VOp)
+    requires Bookmarker.Inv(k, s)
+    requires Bookmarker.Inv(k, s')
+    requires Bookmarker.NextStep(k, s, s', vop, uiop)
+    requires vop.TristateInternalOp?
+    ensures FVM.Next(Ik(k), I(k, s), I(k, s'), uiop)
+  {
+    assert FVM.NextStep(Ik(k), I(k, s), I(k, s'), uiop, FVM.StutterStep);
+  }
+
+  lemma JournalInternalRefines(k: Bookmarker.Constants, s: Bookmarker.Variables, s':Bookmarker.Variables, uiop: UI.Op, vop: VOp)
+    requires Bookmarker.Inv(k, s)
+    requires Bookmarker.Inv(k, s')
+    requires Bookmarker.NextStep(k, s, s', vop, uiop)
+    requires vop.JournalInternalOp?
+    ensures FVM.Next(Ik(k), I(k, s), I(k, s'), uiop)
+  {
+    assert FVM.NextStep(Ik(k), I(k, s), I(k, s'), uiop, FVM.StutterStep);
+  }
+
+  lemma SendFrozenLocRefines(k: Bookmarker.Constants, s: Bookmarker.Variables, s':Bookmarker.Variables, uiop: UI.Op, vop: VOp)
+    requires Bookmarker.Inv(k, s)
+    requires Bookmarker.Inv(k, s')
+    requires Bookmarker.NextStep(k, s, s', vop, uiop)
+    requires vop.SendFrozenLocOp?
+    ensures FVM.Next(Ik(k), I(k, s), I(k, s'), uiop)
+  {
+    assert FVM.NextStep(Ik(k), I(k, s), I(k, s'), uiop, FVM.StutterStep);
+  }
+
+  lemma ForgetOldRefines(k: Bookmarker.Constants, s: Bookmarker.Variables, s':Bookmarker.Variables, uiop: UI.Op, vop: VOp)
+    requires Bookmarker.Inv(k, s)
+    requires Bookmarker.Inv(k, s')
+    requires Bookmarker.NextStep(k, s, s', vop, uiop)
+    requires vop.ForgetOldOp?
+    ensures FVM.Next(Ik(k), I(k, s), I(k, s'), uiop)
+  {
+    assert FVM.NextStep(Ik(k), I(k, s), I(k, s'), uiop, FVM.StutterStep);
+  }
+
+  lemma PushSyncRefines(k: Bookmarker.Constants, s: Bookmarker.Variables, s':Bookmarker.Variables, uiop: UI.Op, vop: VOp)
+    requires Bookmarker.Inv(k, s)
+    requires Bookmarker.Inv(k, s')
+    requires Bookmarker.NextStep(k, s, s', vop, uiop)
+    requires vop.PushSyncOp?
+    ensures FVM.Next(Ik(k), I(k, s), I(k, s'), uiop)
+  {
+    assert FVM.NextStep(Ik(k), I(k, s), I(k, s'), uiop, FVM.PushSyncStep(vop.id));
+  }
+
+  lemma PopSyncRefines(k: Bookmarker.Constants, s: Bookmarker.Variables, s':Bookmarker.Variables, uiop: UI.Op, vop: VOp)
+    requires Bookmarker.Inv(k, s)
+    requires Bookmarker.Inv(k, s')
+    requires Bookmarker.NextStep(k, s, s', vop, uiop)
+    requires vop.PopSyncOp?
+    ensures FVM.Next(Ik(k), I(k, s), I(k, s'), uiop)
+  {
+    assert FVM.NextStep(Ik(k), I(k, s), I(k, s'), uiop, FVM.PopSyncStep(vop.id));
+  }
+
+  lemma RefinesNextStep(k: Bookmarker.Constants, s: Bookmarker.Variables, s':Bookmarker.Variables, uiop: UI.Op, vop: VOp)
+    requires Bookmarker.Inv(k, s)
+    requires Bookmarker.Inv(k, s')
+    requires Bookmarker.NextStep(k, s, s', vop, uiop)
+    ensures FVM.Next(Ik(k), I(k, s), I(k, s'), uiop)
+  {
+    match vop {
+      case SendPersistentLocOp(loc) => { SendPersistentLocRefines(k, s, s', uiop, vop); }
+      case AdvanceOp(uiop, replay) => { AdvanceRefines(k, s, s', uiop, vop); }
+      case CrashOp => { CrashRefines(k, s, s', uiop, vop); }
+      case FreezeOp => { FreezeRefines(k, s, s', uiop, vop); }
+      case TristateInternalOp => { TristateInternalRefines(k, s, s', uiop, vop); }
+      case JournalInternalOp => { JournalInternalRefines(k, s, s', uiop, vop); }
+      case SendFrozenLocOp(loc) => { SendFrozenLocRefines(k, s, s', uiop, vop); }
+      case ForgetOldOp => { ForgetOldRefines(k, s, s', uiop, vop); }
+      case PushSyncOp(id) => { PushSyncRefines(k, s, s', uiop, vop); }
+      case PopSyncOp(id) => { PopSyncRefines(k, s, s', uiop, vop); }
+    }
+  }
+
+  lemma RefinesNext(k: Bookmarker.Constants, s: Bookmarker.Variables, s': Bookmarker.Variables, uiop: UI.Op)
+    requires Bookmarker.Inv(k, s)
+    requires Bookmarker.Next(k, s, s', uiop)
+    ensures Bookmarker.Inv(k, s')
+    ensures FVM.Next(Ik(k), I(k, s), I(k, s'), uiop)
+  {
+    var vop :| Bookmarker.NextStep(k, s, s', vop, uiop);
+    RefinesNextStep(k, s, s', uiop, vop);
+  }
+}
